LLVM_DS_RBT/Delete/Alloc_Optimized/Combine_Opt_Ext.thy
@@ -40,7 +40,6 @@ lemma disjoint_trees_value_map_add_graph [simp]:
         rbt_greater_trans rbt_less_eq_trans)
   done
 
-
 lemma combine_correct_ext':
   "
   llvm_htriple
@@ -55,72 +54,78 @@ lemma combine_correct_ext':
     \<up>(value_of_key res_t = value_of_key l ++ value_of_key r)
   )
   "
-  supply ptr_of_key_simps[simp]
-  supply value_of_key_simps[simp]
-  supply sep_context_pureI[fri_red_rules]
 proof(induction "rbt_of l" "rbt_of r" arbitrary: l r li ri rule: RBT_Impl.combine.induct)
   case 1
   then show ?case
     apply (subst combine_opt.simps)
-    apply vcg
+    apply vcg_vok
     done
 next
   case (2 v va vb vc vd)
   then show ?case
     apply (subst combine_opt.simps)
-    apply vcg
+    apply vcg_vok
     done
 next
   case (3 a k x b c s y d)
   note 3(1)[simplified ctx_def, vcg_rules]
 
   from 3(2-3) show ?case
-    supply RBT_Impl.combine.simps[simp del]
+    supply
+      RBT_Impl.combine.simps[simp del]
+      combine_rbt_sorted[simp]
 
     apply (subst combine_opt.simps)
     apply vcg
     subgoal
       apply resolve_rbt_pat_mat
       subgoal
-        supply rbt_sorted.simps[simp del]
         apply vcg_compat
         apply sepE
-        apply (auto simp add: RBT_Impl.combine.simps)[] 
+         apply (auto simp add: RBT_Impl.combine.simps)[] 
 
         apply sep
-        apply simp
-        apply (rule combine_rbt_sorted)
-        using rbt_sorted.simps apply fast+
-        apply auto[2]
+         apply (simp add: combine_rbt_sorted)
 
-        apply (sepwith auto)
+        apply sep
+        subgoal
+          apply (simp add: ptr_of_key_simps)
+          apply pok_solver
+          done
+        apply sep
+        subgoal
+          apply (simp add: value_of_key_simps)
+          apply vok_solver
+          done
         apply simp
-        apply (sepwith simp)
+        apply sep
         done
       done
     subgoal
-      supply rbt_sorted.simps[simp del]
       apply vcg
-      apply vcg_try_solve
+      apply vcg_compat
+
+      apply sepE (*rbt_of*)
+
        apply (cases "rbt_combine b c")
         apply (auto simp add: RBT_Impl.combine.simps split: color.splits)[2]
-      apply vcg_compat
+
+      apply sep (*sorted*)
+       apply simp
+
       apply sep
+      subgoal
+        apply (simp add: ptr_of_key_simps)
+        apply pok_solver 
+        done
 
-       apply simp
-       apply (rule combine_rbt_sorted)
-      using rbt_sorted.simps apply fast+
-        apply auto[2]
+      apply sep
+      subgoal
+        apply (simp add: value_of_key_simps)
+        apply vok_solver
+        done
 
-      apply sep  
-       apply simp
-       apply (auto simp: rbt_sorted.simps)[1]
-
-      apply sep 
-       supply rbt_sorted.simps[simp]
-       apply vok_solver 
-      apply (metis rbt_greater_simps(2) rbt_sorted.simps(2))
-      apply vok_solver 
+      apply simp
       apply sep
       done
     done
@@ -129,29 +134,36 @@ next
   note 4(1)[simplified ctx_def, vcg_rules]
 
   from 4(2-3) show ?case
-    supply RBT_Impl.combine.simps[simp del]
+    supply
+      RBT_Impl.combine.simps[simp del]
+      combine_rbt_sorted[simp]
 
     apply (subst combine_opt.simps)
     apply vcg
     subgoal
       apply resolve_rbt_pat_mat
-      supply rbt_sorted.simps[simp del]
       apply vcg_compat
+
+      apply sepE
+       apply (auto simp add: RBT_Impl.combine.simps)[] (*rbt_of*)
+
+      apply sep (*sorted*)
+       apply simp 
+
+      apply sep (*pok*)
       subgoal
-        apply sepE
-         apply (auto simp add: RBT_Impl.combine.simps)[] 
-
-        apply sep
-         apply simp
-         apply (rule combine_rbt_sorted)
-        using rbt_sorted.simps apply fast+
-          apply auto[2]
-
-        apply (sepwith auto)
-        apply simp
-        apply (sepwith simp)
-
+        apply (simp add: ptr_of_key_simps)
+        apply pok_solver
         done
+
+      apply sep (*vok*)
+      subgoal
+        apply (simp add: value_of_key_simps)
+        apply vok_solver
+        done
+
+      apply simp
+      apply sep
       done
 
     subgoal
@@ -162,58 +174,94 @@ next
         combine_rbt_less[intro]
       apply vcg
       apply vcg_compat
+ 
       apply sepE
-       apply (cases "rbt_combine b c")
-        apply (auto simp add: RBT_Impl.combine.simps split: color.splits)[2]
+      apply (cases "rbt_combine b c")
+      apply (auto simp add: RBT_Impl.combine.simps split: color.splits)[2]
+   
       apply sep
-
        apply simp
+
       apply sep
+      apply (simp add: ptr_of_key_simps)
       apply pok_solver
+
       apply sep
-       apply vok_solver
+      apply (simp add: value_of_key_simps)
+      apply vok_solver
+      
       apply sep
       done
     done
-  next
-    case (5 va vb vc vd b k x c)
-    note 5(1)[simplified ctx_def, vcg_rules]
-    from 5(2-3) show ?case
-      apply (subst combine_opt.simps)
-      apply vcg
-      apply vcg_compat
-      subgoal
-        supply  
-          rbt_less_trans[intro]
-          rbt_greater_trans[intro]
-          combine_rbt_greater[intro]
-          combine_rbt_less[intro]
+next
+  case (5 va vb vc vd b k x c)
+  note 5(1)[simplified ctx_def, vcg_rules]
+  from 5(2-3) show ?case
+    supply
+      RBT_Impl.combine.simps[simp del]
+      combine_rbt_sorted[simp]
 
-        apply (sepEwith force)
-        apply simp 
-        apply (sepwith simp)
-        done 
-      done
-  next
-    case (6 a k x b va vb vc vd)
-    note 6(1)[simplified ctx_def, vcg_rules]
-    from 6(2-3) show ?case
-      apply (subst combine_opt.simps)
-      apply vcg
-      apply vcg_compat
-      subgoal
-        supply  
-          rbt_less_trans[intro]
-          rbt_greater_trans[intro]
-          combine_rbt_greater[intro]
-          combine_rbt_less[intro]
+    apply (subst combine_opt.simps)
+    apply vcg
+    apply vcg_compat
+    subgoal
+      supply  
+        rbt_less_trans[intro]
+        rbt_greater_trans[intro]
 
-        apply (sepEwith force)
-        apply simp 
-        apply (sepwith simp)
-        done 
-      done
-  qed
+      apply sepE
+       apply (simp add: RBT_Impl.combine.simps)
+
+      apply sep
+       apply simp
+
+      apply sep
+       apply (simp add: ptr_of_key_simps)
+       apply pok_solver
+
+      apply sep
+       apply (simp add: value_of_key_simps)
+       apply vok_solver
+
+      apply simp 
+      apply sep
+      done 
+    done
+next
+  case (6 a k x b va vb vc vd)
+  note 6(1)[simplified ctx_def, vcg_rules]
+  from 6(2-3) show ?case
+    supply
+      RBT_Impl.combine.simps[simp del]
+      combine_rbt_sorted[simp]
+
+    apply (subst combine_opt.simps)
+    apply vcg
+    apply vcg_compat
+    subgoal
+      supply  
+        rbt_less_trans[intro]
+        rbt_greater_trans[intro]
+
+      apply sepE
+       apply (simp add: RBT_Impl.combine.simps)
+
+      apply sep
+       apply simp
+
+      apply sep
+       apply (simp add: ptr_of_key_simps)
+       apply pok_solver
+
+      apply sep
+       apply (simp add: value_of_key_simps)
+       apply vok_solver
+
+      apply simp 
+      apply sep
+      done 
+    done
+qed
 
 lemmas combine_correct_ext[vcg_rules] = combine_correct_ext'[simplified ctx_def]
 
